src/tactics/FStar.Tactics.Basic.fsti
@@ -62,7 +62,7 @@ val unshelve               : term -> tac unit
 val unquote                : typ -> term -> tac term
 val norm                   : list EMB.norm_step -> tac unit
 val norm_term_env          : env -> list EMB.norm_step -> term -> tac term
-val norm_binder_type       : list EMB.norm_step -> binder -> tac unit
+val norm_binder_type       : list EMB.norm_step -> RD.binding -> tac unit
 val intro                  : unit -> tac RD.binding
 val intro_rec              : unit -> tac (RD.binding * RD.binding)
 val rename_to              : RD.binding -> string -> tac RD.binding
